Utils.dfy
@@ -14,4 +14,25 @@ module Utils {
   {
     if a <= b then a else b
   }
+
+  function maps<P,Q> (xs: seq<P>, f:P->Q): seq<Q>
+    ensures |xs| == |maps(xs, f)|
+    ensures forall i :: 0 <= i < |xs| ==> f(xs[i]) == maps(xs, f)[i]
+  {
+    if |xs| == 0 then [] else [f(xs[0])] + maps(xs[1..], f)
+  }
+
+  function filter<P> (xs: seq<P>, p: P -> bool): seq<P>
+    ensures |xs| <= |maps(xs, p)|
+    ensures forall i :: 0 <= i < |xs| ==> (p(xs[i]) ==> xs[i] in filter(xs, p))
+    ensures forall i :: 0 <= i < |filter(xs,p)| ==> p(filter(xs,p)[i])
+  {
+    if |xs| == 0 then [] else (if p(xs[0]) then [xs[0]] else []) + filter(xs[1..], p)
+  }
+
+
+  function foldRight<P,Q> (xs: seq<P>, init: Q, f: (P,Q) -> Q): Q
+  {
+    if |xs| == 0 then init else foldRight(xs[1..], f(xs[|xs|-1], init), f)
+  }
 }
